 \documentclass[a4paper,12pt]{report}

%Packages Used
\usepackage{amssymb,latexsym,amsmath}     % Standard packages
\usepackage{setspace}
\usepackage{sectsty}
\usepackage{titlesec}
\usepackage{hyperref}
\usepackage{bookmark}
\usepackage{graphics,graphicx}
\usepackage{tikz}
\usepackage{mathtools}
\usepackage{graphicx}
\usepackage{esvect}

\DeclarePairedDelimiter\abs{\lvert}{\rvert}%
\DeclarePairedDelimiter\norm{\lVert}{\rVert}%


\bookmarksetup{
  numbered,
  open
}
\renewcommand*{\thesection}{\arabic{section}}
\onehalfspacing

%Margins
\addtolength{\textwidth}{1.0in}
\addtolength{\textheight}{1.00in}
\addtolength{\evensidemargin}{-0.75in}
\addtolength{\oddsidemargin}{-0.75in}
\addtolength{\topmargin}{-.50in}

%%%%%%%%%%%%%%%%%%%%%%%%%%%%%% 
% Theorem/Proof Environments %
%%%%%%%%%%%%%%%%%%%%%%%%%%%%%%
\newtheorem{theorem}{Theorem}
\newenvironment{proof}{\noindent{\bf Proof:}}{$\hfill \Box$ \vspace{10pt}}
\sectionfont{\fontsize{12}{15}\selectfont}
\titlespacing*{\section}{0.5pt}{0.25\baselineskip}{0.25\baselineskip}

\begin{document}
\noindent
Yufei Lin

\noindent
Problem Set 4

\noindent
Oct \(24^{th}\) 2019

\begin{center}
\textbf{Problem Set 4}
\end{center}

\noindent
\textbf{Chapter 5 \#12}

\noindent
\textbf{(a) Proof }

\noindent
Suppose $\forall x, f(x)\leq g(x)$, and both $\displaystyle{\lim_{x\to a}}f(x) = L$ and $\displaystyle{\lim_{x\to a}}g(x) = M$. Then we know, $\displaystyle{\lim_{x\to a}}g(x)-\displaystyle{\lim_{x\to a}}f(x)=\displaystyle{\lim_{x\to a}}(g(x)-f(x)) = M-L$. Since $(g(x)-f(x))\geq 0$, then $\displaystyle{\lim_{x\to a}}(g(x)-f(x))$ is a limit of a positive number or 0. Thus,  $\displaystyle{\lim_{x\to a}}g(x)-\displaystyle{\lim_{x\to a}}f(x)=\displaystyle{\lim_{x\to a}}(g(x)-f(x))\geq 0$. Therefore, $\displaystyle{\lim_{x\to a}}g(x)\geq \displaystyle{\lim_{x\to a}}f(x)$.\\

\noindent
\textbf{(b) Answer }

\noindent
If $\exists d >0$ such that $\forall x, |x-a|<d$, $f(x)\leq g(x)$ and both limit exists at $a$, then $\displaystyle{\lim_{x\to a}}f(x)\leq \displaystyle{\lim_{x\to a}}g(x)$.\\

\noindent
\textbf{(c) Counter Example}

\[  f(x)= \left\{
\begin{array}{ll}
      |x| & x\neq 0 \\
      1 & x = 0 \\
\end{array} 
\right. \]

\[  g(x)= \left\{
\begin{array}{ll}
      -|x| & x\neq 0 \\
      -1 & x = 0 \\
\end{array} 
\right. \]

\noindent
Thus, $f(x)<g(x)$ and $\displaystyle{\lim_{x\to a}}g(x) = \displaystyle{\lim_{x\to a}}f(x) = 0$.\\

\noindent
\textbf{Chapter 5 \#13}

\noindent
\textbf{Chapter 5 \#17}

\noindent
\textbf{Chapter 5 \#19}
\end{document}