 \documentclass[a4paper,12pt]{report}

%Packages Used
\usepackage{amssymb,latexsym,amsmath}     % Standard packages
\usepackage{setspace}
\usepackage{sectsty}
\usepackage{titlesec}
\usepackage{hyperref}
\usepackage{bookmark}
\usepackage{graphics,graphicx}
\usepackage{tikz}
\usepackage{mathtools}
\usepackage{graphicx}
\usepackage{esvect}

\DeclarePairedDelimiter\abs{\lvert}{\rvert}%
\DeclarePairedDelimiter\norm{\lVert}{\rVert}%
\DeclarePairedDelimiter\ceil{\lceil}{\rceil}
\DeclarePairedDelimiter\floor{\lfloor}{\rfloor}

\usepackage{url,graphicx,enumitem}


%   Article style enumerate

\renewcommand{\labelenumi}{\theenumi.}

\newcommand{\R}{\mathbb{R}}
\newcommand{\Z}{\mathbb{Z}}
\newcommand{\N}{\mathbb{N}}

\newcommand{\bull}{\ensuremath{\bullet}}

\newcommand{\vc}[1]{\vec{#1}}

\newcommand{\transpose}{\mathsf{T}}

\newcommand{\lcm}{\mathrm{lcm}}
\newcommand{\ud}{\mathrm{d}}

\bookmarksetup{
  numbered,
  open
}
\renewcommand*{\thesection}{\arabic{section}}
\onehalfspacing

%Margins
\addtolength{\textwidth}{1.0in}
\addtolength{\textheight}{1.00in}
\addtolength{\evensidemargin}{-0.75in}
\addtolength{\oddsidemargin}{-0.75in}
\addtolength{\topmargin}{-.50in}

%%%%%%%%%%%%%%%%%%%%%%%%%%%%%% 
% Theorem/Proof Environments %
%%%%%%%%%%%%%%%%%%%%%%%%%%%%%%
\newtheorem{theorem}{Theorem}
\newenvironment{proof}{\noindent{\bf Proof:}}{$\hfill \Box$ \vspace{10pt}}
\sectionfont{\fontsize{12}{15}\selectfont}
\titlespacing*{\section}{0.5pt}{0.25\baselineskip}{0.25\baselineskip}


\begin{document}
\noindent
Yufei Lin

\noindent
Problem Set 8

\noindent
Nov \(25^{th}\) 2019

\begin{center}
\textbf{Problem Set 8}
\end{center}

\noindent
\textbf{Question 1}

\noindent
Suppose that $f:[a,b]\rightarrow\mathbb{R}$, is integrable, and suppose that $m=inf\{f(x):x\in [a,b]\}$ and $M=sup\{f(x):x\in [a,b]\}$. Then, we have $m(b-a)\leq \int_{a}^{b}f\leq M(b-a)$.

\noindent
\textbf{Proof: }

\noindent
Lemma: Suppose $f:[a,b]\rightarrow\mathbb{R}$ is integrable and suppose that $P$ is any partition $[a,b]$. Then we have $L(f,P)\leq \int_{a}^{b}f\leq U(f,P)$.

\noindent
Proof of Lemma:

\noindent
We will prove this lemma from two parts:

\noindent
First, we prove that $L(f,P)\leq \int_{a}^{b}f$.

\noindent
Since $f$ is integrable, then we know $sup\{L(f,P)|P, \text{a partition in range }[a,b]\}=\int_{a}^{b}f$. And let $A=\{L(f,P)|P, \text{a partition in range }[a,b]\}$. Then $supA$ is the least upper bound of $A$. Let $y=supA$, then $\forall x \in A, x\leq y$. Then, because we have $y=\int_{a}^{b}f$, $\forall x\in A, x\leq y=\int_{a}^{b}f$. Thus, $L(f,P)\leq \int_{a}^{b}f$. 

\noindent
Then, we prove that $\int_{a}^{b}f\leq U(f,P)$. 

\noindent
Since $f$ is integrable, we know $inf\{U(f,P)|P, \text{a partition in range }[a,b]\}=\int_{a}^{b}f$. And let $B=\{U(f,P)|P, \text{a partition in range }[a,b]\}$. Let $z=infB$, then $\forall x\in B, z\leq x$. Therefore, since we have $U(f,P)\geq \int_{a}^{b}f$. 

\noindent
Thus, $L(f,P)\leq \int_{a}^{b}f\leq U(f,P)$.

\noindent
From the definition, $L(f,P)=\sum_{i=1}^{n}m_i(t_i-t_{i-1})$ and $U(f,P)=\sum_{i=1}^{n}M_i(t_i-t_{i-1})$. In this case, we have the partition $P$ as $[a,b]$ meaning there's only one pair of $m$ and $M$, and $t_i = b$, $t_{i-1}=a$. Therefore, we have $L(f,P)=m(b-a)$ and $U(f,P)=M(b-a)$. Thus, from the lemma we know that $m(b-a)\leq \int_{a}^{b}f\leq M(b-a)$. \\

\noindent
\textbf{Question 2}

\noindent
Prove that the function $f:[-1,1]\to\R$,
defined by 
\[
f(n) = \begin{cases} 1 &\mbox{if } x\geq 0 \\
0 & \mbox{if } x<0 \end{cases},
\]
is integrable on $[-1,1]$. 

\noindent
\textbf{Proof:}

\noindent
At first we choose the partition $P=\{-1,0,1\}$. Then, by definition, $L(f,P)=\sum_{i=1}^{n}m_i(t_i-t_{i-1})$ and $U(f,P)=\sum_{i=1}^{n}M_i(t_i-t_{i-1})$. Therefore, we have, 
\begin{align*}
L(f,P)&=\sum_{i=1}^{2}m_i(t_i-t_{i-1})\\
&=m_1\cdot{(t_1-t_0)}+m_2\cdot{(t_2-t_1)}\\
&=0\cdot{(-0+1)}+1\cdot{(1-0)}\\
&=1
\end{align*}
and 
\begin{align*}
U(f,P)&=\sum_{i=1}^{2}M_i(t_i-t_{i-1})\\
&=M_1\cdot{(t_1-t_0)}+M_2\cdot{(t_2-t_1)}\\
&=1\cdot{(-0+1)} + 1\cdot{(1-0)}\\
&=2
\end{align*}

\noindent
Thus, we have $1\leq \int_{a}^{b}f\leq 2$.

\noindent
Then, suppose $f$ is not integrable on $[-1,1]$. Therefore, $\forall \epsilon\in \mathbb{R}, \epsilon>0$ such that if $P=\{-1,-\epsilon,1\},$ then, $L(f,P)<U(f,P)$. Therefore, we have 
\begin{align*}
U(f,P)&=\sum_{i=1}^{2}M_i(t_i-t_{i-1})\\
&=M_1\cdot{(t_1-t_0)}+M_2\cdot{(t_2-t_1)}\\
&=0\cdot{(-\epsilon+1)}+1\cdot{(1+\epsilon)}\\
&=1+\epsilon
\end{align*}
Then, $1+\epsilon\geq \int_{a}^{b}f$. Also we have $1\leq \int_{a}^{b}f$. Therefore, $0\leq \int_{a}^{b}f-1\leq \epsilon$. Since $f$ is not integrable, then we have $0< \int_{a}^{b}f-1$. Let $\delta =\int_{a}^{b}f-1, \delta>0$. Since $\epsilon>0$, therefore, $\exists \epsilon, \delta>\epsilon>0$. Thus, $\exists \epsilon, \int_{a}^{b}f-1>\epsilon>0$. Then, we have $\int_{a}^{b}f>1+\epsilon$, which is a contradiction. Thus, $f$ is integrable on $[-1,1]$.  \\

\noindent
\textbf{Question 3}

\noindent
Suppose that $f:[a,b]\to\R$,
is bounded. Then $f$ is integrable on $[a,b]$
if, and only if, for every $\epsilon>0$, there
exists a partition $P$ of $[a,b]$ such
that
\[
U(f,P)-L(f,P)<\epsilon.
\]

\noindent
\textbf{Proof: }

\noindent
Suppose $\forall \epsilon > 0U(f,P)-L(f,P)<\epsilon $, then we know by definition of $sup\{L(f,P)\}$ and $inf\{U(f,P)\}$ that $sup\{L(f,P\}\geq L(f,P)$, $inf\{U(f,P)\}\leq U(f,P)$ and $inf\{U(f,P)\}\geq sup\{L(f,P\}$. Thus, $0\leq inf\{U(f,P)\}-sup\{L(f,P)\}\leq U(f,P)-L(f,P)<\epsilon$. Let $\delta=inf\{U(f,P)\}-sup\{L(f,P)\}$. Suppose $\delta > 0$. Since $\forall \epsilon>0 \delta<\epsilon$. But we have $a=\delta-0=\delta$ such that if $\epsilon<a=\delta$, then, we have $0<\epsilon<\delta$ and we reach a contradiction. Therefore, $\delta=0$. Thus, $inf\{U(f,P)\} = sup\{L(f,P)\}$. Then, $f$ is integrable on $[a,b]$, based on the definition. 

\noindent
Conversely, suppose $f$ is integrable on $[a,b]$. Therefore, we know that $inf\{U(f,P)\} = sup\{L(f,P)\}$. Also, we know that  $sup\{L(f,P)\}\geq L(f,P)$ and $inf\{U(f,P)\}\leq U(f,P)$. Therefore, $0=inf\{U(f,P)\}-sup\{L(f,P)\}\leq U(f,P)-L(f,P)$. Suppose $\exists \epsilon>0$ such that $\forall P, U(f,P)-L(f,P)>\epsilon$. Therefore, we would have $inf\{U(f,P)\}-sup\{L(f,P)\} = 0>\epsilon$. Then, we have a contradiction. Therefore, we know that if $f$ is integrable on $[a,b]$, then $\forall \epsilon >0$ there
exists a partition $P$ of $[a,b]$ such
that
$
U(f,P)-L(f,P)<\epsilon.
$\\

\noindent
\textbf{Question 4}

\noindent
Use the theorem you proved in 
question \#3 to solve 
question \#2 again 
in a slightly different way. (It 
should be easier this way, but it is
worth doing it both ways.)

\noindent
\textbf{Proof: }

\noindent
Suppose $P=\{t_0,t_1,...,t_n\}$ is a partition of $[-1,1]$ with $t_j = 0, j \in \mathbb{Z}, j \in [0,n]$. Then, we have when $i<j$, $m_i=M_i=0$ and if $i>j$, we have $m_i=M_i=1$, $m_j=0$ and $M_j=1$. Since we have:
\begin{align*}
L(f,P_n)&=\sum_{i=1}^{j-1}m_i(t_i-t_{i-1})+m_j(t_j-t_{j-1})+\sum_{i=j+1}^{n}m_i(t_i-t_{i-1})\\
U(f,P_n)&=\sum_{i=1}^{j-1}M_i(t_i-t_{i-1})+M_j(t_j-t_{j-1})+\sum_{i=j+1}^{n}M_i(t_i-t_{i-1})\\
\end{align*}
Then, $U(f,P)-L(f,P)=t_j-t_{j-1}$. Suppose $\epsilon >0$ and assume $P$ with an interval such that $t_i-t_{i-1}<\epsilon$, for each $i$. Thus, we have $t_j-t_{j-1}<\epsilon$ and therefore, $f$ is integrable. \\

\noindent
\textbf{Chpater 13. \#1}

\noindent
Prove that $\int_{0}^{b}x^3dx=\frac{b^4}{4}$, by considering partitions into $n$ equal intervals. 

\noindent
\textbf{Proof: }

\noindent
Since we are going to have a partition with $n$ intervals, then we would have $P=\{t_0,t_1,...,t_n\}$ with $t_0=0, t_i=i\cdot{\frac{b}{n}}$. Then, we have
\begin{align*}
L(f,P_n)&=\sum_{i=1}^{n}t_{i-1}^{3}(t_i-t_{i-1})\\
&=\sum_{i=1}^{n}(\frac{(i-1)\cdot{b}}{n})^{3}\cdot{\frac{b}{n}}\\
&=(\frac{b}{n})^4\cdot{\sum_{i=1}^{n}(i-1)^{3}}\\
&=(\frac{b}{n})^4\cdot{\sum_{j=0}^{n-1}j^{3}}
\end{align*}
\begin{align*}
U(f,P_n)&=\sum_{i=1}^{n}t_{i}^{3}(t_i-t_{i-1})\\
&=\sum_{i=1}^{n}(\frac{i\cdot{b}}{n})^{3}\cdot{\frac{b}{n}}\\
&=(\frac{b}{n})^4\cdot{\sum_{i=1}^{n}i^{3}}
\end{align*}
From the previous question Chapter 2 \#6, we know that $\sum_{i=1}^{n}i^3=\frac{n^4}{4}+\frac{n^3}{2}+\frac{n^2}{2}$, and the equation could be written:
\begin{align*}
L(f,P_n)&=(\frac{b}{n})^4\cdot{(\frac{(n-1)^4}{4}+\frac{(n-1)^3}{2}+\frac{(n-1)^2}{4})}\\
&=(\frac{b}{n})^4\cdot{\frac{1}{4}}((n-1)^4+2(n-1)^3+(n-1)^2)\\
&=\frac{b^4}{4}\cdot{(\frac{(n-1)^4}{n^4}+\frac{2(n-1)^3}{n^4}+\frac{(n-1)^2}{n^4})}\\
U(f,P_n)&=(\frac{b}{n})^4\cdot{(\frac{n^4}{4}+\frac{n^3}{2}+\frac{n^2}{4})}\\
&=(\frac{b}{n})^4\cdot{\frac{1}{4}}(n^4+2n^3+n^2)\\
&=\frac{b^4}{4}\cdot{(1+\frac{2}{n}+\frac{1}{n^2})}
\end{align*}
Since $n\geq 1, n\in \mathbb{N}$, therefore, we know when $n$ gets very large both $U(f,P_n)$ and $L(f,P_n)$ are close to $\frac{b^4}{4}$. At the same time, we find that \[U(f,P_n)-L(f,P_n)=\frac{b^4}{4}(\frac{2n^3-1}{n^4})\] which is a positive number. And we can make this difference as small as possible, by theorem 2, this function is integrable. Therefore, we have $U(f,P_n)\geq \frac{b^4}{4} \geq L(f,P_n)$. Thus, $\int_{0}^{b}x^3dx=\frac{b^4}{4}$. \\

\noindent
\textbf{Chpater 13. \#13}

\noindent
\textbf{(a)} Prove that if $f$ is integrable on $[a,b]$ and $f(x)\geq 0$ for all $x$ in $[a,b]$, then $\int_{a}^{b}f\geq 0$. 

\noindent
\textbf{Proof: }

\noindent
Since $f$ is integrable on $[a,b]$, then we have $U(f,P_n)\geq \int_{a}^{b}f \geq L(f,P_n)$. Also, based on the definition, we have:
\begin{align*}
L(f,P_n)&=\sum_{i=1}^{n}f(t_{i-1})(t_i-t_{i-1})\\
U(f,P_n)&=\sum_{i=1}^{n}f(t_{i})(t_i-t_{i-1})\\
\end{align*}
Also, because $f(x)\geq 0, \forall x\in [a,b]$ and $t_{i-1}\in[a,b], \forall i\in \mathbb{N}, i\leq n$, then $f(t_{i-1})\geq 0$. Also, because the definition of $t_i$ guarantees, $t_i>t_{i-1}$, then $t_i-t_{i-1}>0$ Therefore, let $q_i=f(t_{i-1})(t_i-t_{i-1})$, since both $f(t_{i-1})$ and$(t_i-t_{i-1})$ are greater than or equal to $0$. We have $q_i\geq 0$. Similarly, because $t_i\in [a,b], \forall i\in \mathbb{N}, i\leq n$, then $f(t_i)\geq 0$. Let $p_i=f(t_{i})(t_i-t_{i-1})$. Because both $f(t_{i-1})$ and$(t_i-t_{i-1})$ are both greater than or equal to $0$. Then, $p_i\geq 0$. Thus, we have $U(f,P_n)\geq \int_{a}^{b}f \geq L(f,P_n)\geq 0$. Thus, $\int_{a}^{b}f \geq 0$.\\

\noindent
\textbf{(b)}Prove that if $f$ and $g$ are both integrable on $[a,b]$ and $f(x)\geq g(x), \forall x\in [a,b]$, then $\int_{a}^{b}f\geq \int_{a}^{b}g$. 

\noindent
\textbf{Proof:}

\noindent
Suppose $f$ and $g$ are both integrable on $[a,b]$ and $f(x)\geq g(x), \forall x\in [a,b]$. Then, we know that $f(x)-g(x)\geq 0$. Thus, $(f-g)(x)\geq 0, \forall x\in [a,b]$. Furthermore, from theorem 5, we know that for any two functions that are integrable at the same range, we have $\int_{a}^{b}f+\int_{a}^{b}g=\int_{a}^{b}(f+g)$. Furthermore, from theorem 6 we know that $\int_{a}^{b}cg=c\cdot{\int_{a}^{b}g}$. Thus, $\int_{a}^{b}-g=-\int_{a}^{b}g$. Then, we have $\int_{a}^{b}f-\int_{a}^{b}g=\int_{a}^{b}(f-g)$. Let $L(x)=(f-g)(x)$, then $\int_{a}^{b}(f-g)=\int_{a}^{b}L$ and from the previous theorem that if $f$ is integrable on $[a,b]$ and $f(x)\geq 0$ for all $x$ in $[a,b]$, then $\int_{a}^{b}f\geq 0$. We know that $\int_{a}^{b}L\geq 0$. Thus $\int_{a}^{b}f-\int_{a}^{b}g=\int_{a}^{b}(f-g)=\int_{a}^{b}L\geq 0$. Therefore, $\int_{a}^{b}f\geq \int_{a}^{b}g$.\\

\noindent
\textbf{Chpater 13. \#20}

\noindent
Suppose that $f$ is nondecreasing on $[a,b]$. Notice that $f$ is automatically bounded on $[a,b]$, because $f(a)\geq f(x)\geq f(b), \forall x\in [a,b]$.

\noindent
\textbf{(a)}If $P=\{t_0,t_1,...,t_n\}$ is a partition of $[a,b]$, then what is $L(f,P)$ and $U(f,P)$

\noindent
\textbf{Answer: }

\noindent
By definition of $L(f,P)$ and $U(f,P)$, we have the following:
\begin{align*}
L(f,P_n)&=\sum_{i=1}^{n}f(t_{i-1})(t_i-t_{i-1})\\
U(f,P_n)&=\sum_{i=1}^{n}f(t_{i})(t_i-t_{i-1})\\
\end{align*}

\noindent
\textbf{(b)}Suppose that $t_{i}-t_{i-1}=\delta$ for each $i$. Prove that $U(f,P_n)-L(f,P_n)=\delta\cdot(f(b)-f(a))$.

\noindent
\textbf{Proof: }

\noindent
Suppose $t_{i}-t_{i-1}=\delta$ for each $i$. Therefore, we know that 
\begin{align*}
U(f,P_n)-L(f,P_n)&=\sum_{i=1}^{n}f(t_{i})(t_i-t_{i-1})-\sum_{i=1}^{n}f(t_{i-1})(t_i-t_{i-1})\\
&=\sum_{i=1}^{n}(f(t_{i})\cdot{\delta})-\sum_{i=1}^{n}(f(t_{i-1})\cdot{\delta})\\
&=\delta\cdot{(\sum_{i=1}^{n}(f(t_{i})-\sum_{i=1}^{n}(f(t_{i-1})))}\\
&=\delta\cdot{(\sum_{i=1}^{n}(f(t_{i})-f(t_{i-1}))}\\
&=\delta\cdot{((f(t_1)-f(t_0))+(f(t_2)-f(t_1))+...+(f(t_n)-f(t_{n-1})))}\\
&=\delta\cdot{(f(t_n)-f(t_0))}\\
&=\delta\cdot{(f(b)-f(a))}
\end{align*}
 
\noindent
\textbf{(c)}Prove $f$ is integrable.

\noindent
\textbf{Proof: }

\noindent
Since we have $U(f,P_n)-L(f,P_n)=\delta\cdot{(f(b)-f(a))}$ and $\delta$ is arbitrary and $f(b)-f(a)$ is given because we know $f$ and both $f(a)$ and $f(b)$ exist. Therefore, we could have $\forall \epsilon>0, \exists \delta<\frac{\epsilon}{f(b)-f(a)}$. Then, we have $\delta\cdot{(f(b)-f(a))}<\epsilon$ and $U(f,P_n)-L(f,P_n)<\epsilon$. \\

\noindent
\textbf{(d)} Give an example of a nondecreasing function on $[0,1]$ which is discontinuous at infinitely many points. 

\noindent
\textbf{Example: }

 $y =
    \begin{cases}
      0 & x=0\\
      \frac{1}{\floor*{\frac{1}{x}}} & 0<x<1\\
      1 & x=1
    \end{cases}  $\\
    
\noindent
\textbf{Chapter 13 \#23}

\noindent
\textbf{(a)}Prove that if $f$ is integrable on $[a,b]$ and $m\leq f(x)\leq M$ for all $x$ in $[a,b]$, then $\int_a^bf(x)dx=(b-a)\mu$, for some number $\mu$ with $m\leq \mu\leq M$.

\noindent
\textbf{Proof:}

\noindent
From Theorem 7, we have if $f$ is integrable on $[a,b]$ and $m\leq f(x)\leq M$, then $m(b-a)\leq \int_{a}^{b}f\leq M(b-a)$. Let $q = \int_{a}^{b}f$. Then, $m(b-a)\leq q\leq M(b-a)$. 

\noindent
Assume $b-a=0$, then we have $0\leq q \leq 0$, meaning $q=0$. We also know that every number is a factor of $0$. Therefore, the assumption holds that if $f$ is integrable on $[a,b]$ and $m\leq f(x)\leq M$ for all $x$ in $[a,b]$, then $\int_a^bf(x)dx=(b-a)\mu$, for some number $\mu$ with $m\leq \mu\leq M$.

\noindent
Let $(b-a)>0$, we have $m\leq \frac{q}{(b-a)}\leq M$. Thus, let $\mu = \frac{q}{(b-a)}$, then $m\leq \mu\leq M$ and $q=\mu\cdot{(b-a)}=\int_{a}^{b}f$. Thus, if $f$ is integrable on $[a,b]$ and $m\leq f(x)\leq M$ for all $x$ in $[a,b]$, then $\int_a^bf(x)dx=(b-a)\mu$, for some number $\mu$ with $m\leq \mu\leq M$.\\

\noindent
\textbf{(b)}Prove that if $f$ is continuous on $[a,b]$, then $\int_a^bf(x)dx=(b-a)f(\xi)$, for some number $\xi$ in $[a,b]$. and show by an example that continuity is essential.

\noindent
\textbf{Proof: }

\noindent
From Chapter 7, theorem 3 and 6 we know that because $f$ is bounded in $[a,b]$, then $\exists K\geq f(x), \forall x \in [a,b]$ and $\exists O\leq f(x), \forall x \in [a,b]$, where in this case $K= M$ and $O=m$. Thus, we know that $\exists a' \in [a,b]$ such that $f(a')=m$ and $\exists b' \in [a,b]$ such that $f(b')=M$. From Chapter 7, theorem 4, we know that if $f$ is continuous on $[a,b]$, and $f(a)<c<f(b)$, then there is some $x$ in $[a,b]$ such that $f(x) = c$. Therefore, from the previous problem we have shown that $\int_a^bf(x)dx=(b-a)\mu$, for some number $\mu$ with $m=f(a')<\mu<f(b')=M$, then we know that from this theorem, since $f$ is continuous, we have there exists $\xi \in [a',b']$ such that $f(\xi )=\mu$.Also, because $[a',b']\subseteq [a,b]$. Therefore, $\xi \in [a,b]$. Thus, the statement holds.
This continuous is essential because if we have a $g(x)=
\begin{cases}
f(x) & x\neq \xi\\
k, k\in \mathbb{R}, k\neq f(\xi) &x=\xi
\end{cases}$, then this assumption does not hold since there is no $f(x)=\mu$. 
\\

\noindent
\textbf{(c)}More generally suppose that $f$ is continuous on $[a,b]$ and that $g$ is integrable and nonnegative on $[a,b]$. Prove that $\int_a^bf(x)g(x)dx=f(\xi)\int_a^bg(x)dx$ for some number $\xi$ in $[a,b]$. This is called the Mean Value Theorem in Integrals. 

\noindent
\textbf{Proof: }

\noindent
From the assumption $m\leq f(x)\leq M$, we know $mg(x)\leq f(x)g(x)\leq Mg(x)$. Therefore, we have $\int_a^bmg(x)dx\leq  \int_a^bf(x)g(x)dx \leq \int_a^bMg(x)dx$. And from theorem 6, we have this inequality rewritten as $m\int_a^bg(x)dx\leq  \int_a^bf(x)g(x)dx \leq M\int_a^bg(x)dx$. Let $q =\int_a^bf(x)g(x)dx$, then we have $m\int_a^bg(x)dx\leq  q \leq M\int_a^bg(x)dx$.

\noindent
Assume $\int_a^bg(x)dx=0$, then we have $0\leq q\leq 0$ and therefore, $q =0$. Thus, $\forall x \in [a,b], f(x)\cdot\int_a^bg(x)dx=0$ and therefore holds the claim that $\int_a^bf(x)g(x)dx=f(\xi)\int_a^bg(x)dx$ for some number $\xi$ in $[a,b]$.

\noindent
Furthermore, if $\int_a^bg(x)dx>0$, then we have $m\leq \frac{q}{\int_a^bg(x)dx}\leq M$. Let $\mu = \frac{q}{\int_a^bg(x)dx}$. Thus, we know from part (b) that $\exists \xi$ such that $f(\xi)=\mu$ and $f(\xi)\int_a^bg(x)dx=\int_a^bf(x)g(x)dx$.\\

\noindent
\textbf{(d)}Deduce the same result if $g$ is integrable and nonpositive on $[a,b]$.

\noindent
\textbf{Proof: }

\noindent
Since we have $g(x)$ as a nonpositive number, then we multiply the original inequality $m\leq f(x)\leq M$ by $-g(x)$. Then, we have $-mg(x)\leq -f(x)g(x)\leq -Mg(x)$. Therefore, we know that $\int_a^b-mg(x)dx\leq  \int_a^b-f(x)g(x)dx \leq \int_a^b-Mg(x)dx$. Then, we know $m\int_a^b-g(x)dx\leq  \int_a^b-f(x)g(x)dx \leq M\int_a^b-g(x)dx$. 

\noindent
Similarly from previous proof, if $\int_a^b-g(x)dx=0$, then we know that $\int_a^b-f(x)g(x)dx=0$. Thus, we also have $\forall x, x\in[a,b], f(x)\int_a^bg(x)dx=0$. And therefore, the statement holds.

\noindent
Furthermore, we have $\int_a^b-g(x)dx>0$. Then, let $\mu = \frac{\int_a^b-f(x)g(x)dx}{\int_a^b-g(x)dx}$. We know that $m< \mu <M$. From part(b) we know that there exists $\xi$ such that $f(\xi)=\mu$ and therefore, the statement holds.\\

\noindent
\textbf{(e)}Show that one of these two hypotheses for $g$ is essential. 

\noindent
\textbf{Answer: }

\noindent
If $g(x)=x^3$ on $[-1,1]$ and $f(x)=x$, then we have 
\begin{align*}
\int_{-1}^1f(x)g(x)dx&=\int_{-1}^1x^4dx\\
&=\frac{x^5}{4}]_{-1}^{1}\\
&=\frac{1}{2}
\end{align*}

\noindent
Then, we have 
\begin{align*}
\int_{-1}^1f(x)dx&=\frac{x^2}{2}]_{-1}^1\\
&=0\\
\int_{-1}^1g(x)dx&=\frac{x^4}{3}]_{-1}^1\\
&=\frac{2}{3}
\end{align*}
Therefore, we have $\mu =0$ and $\mu\cdot \int_{-1}^1g(x)dx=0\neq \frac{1}{2}$, and the statement does not hold. 
\end{document}